Added simple phase1a performance lemma

ironfleet/src/Dafny/Distributed/Protocol/RSL/PerformanceProof/PerformanceProof.i.dfy
@@ -7,6 +7,76 @@ include "../Replica.i.dfy"
 
 include "TimestampedRslSystem.i.dfy"
 
+include "../CommonProof/Constants.i.dfy"
+
 module RslPerformanceProof_i {
-  import opened TimestampedRslPerformanceProof_i
+import opened TimestampedRslPerformanceProof_i
+import opened CommonProof__Constants_i
+
+predicate RslAssumption(s:TimestampedRslState)
+{
+  |s.t_replicas| > 0
+}
+
+predicate RslConsistency(s:TimestampedRslState)
+{
+  ConstantsAllConsistentInv(UntimestampRslState(s))
+}
+
+predicate ViewAlwaysZero(s:TimestampedRslState)
+{
+  && (forall idx:: 0 <= idx < |s.t_replicas|
+    ==>
+    s.t_replicas[idx].v.replica.proposer.election_state.current_view.proposer_id == 0
+    )
+}
+
+predicate AlwaysInvariant(s:TimestampedRslState)
+{
+  && ViewAlwaysZero(s)
+}
+
+predicate InitInvariant(s:TimestampedRslState)
+  requires RslConsistency(s)
+{
+  && (forall idx:: 0 <= idx < |s.t_replicas|
+    ==> 
+    TimeEq(s.t_replicas[idx].ts, TimeZero())
+    )
+
+  && (0 < |s.t_replicas| ==>
+  var p := s.t_replicas[0].v.replica.proposer;
+    && p.current_state == 0
+    && BalLt(p.max_ballot_i_sent_1a, p.election_state.current_view)
+  )
+}
+
+predicate Phase1Invariant(s:TimestampedRslState)
+  requires RslConsistency(s)
+{
+  && (0 < |s.t_replicas| ==>
+    && TimeEq(s.t_replicas[0].ts, L)
+  )
+  && (0 < |s.t_replicas| ==>
+    && s.t_replicas[0].v.replica.proposer.current_state == 1
+  )
+}
+
+lemma Init(s:TimestampedRslState, s':TimestampedRslState)
+  requires RslAssumption(s);
+  requires ViewAlwaysZero(s)
+  requires RslConsistency(s);
+  requires RslConsistency(s');
+
+  requires s.t_environment.nextStep.LEnvStepHostIos?;
+  requires s.t_environment.nextStep.actor == s.constants.config.replica_ids[0];
+  requires s.t_environment.nextStep.nodeStep == RslStep(1);
+
+  requires TimestampedRslNextOneReplica(s, s', 0, s.t_environment.nextStep.ios);
+
+  requires InitInvariant(s)
+  ensures Phase1Invariant(s')
+{
+}
+
 }
